id well-typed

Cm/Questions/PiListApp2.lean
@@ -62,6 +62,7 @@ Core elements so far:
 - composition (cons)
 - pairs ⟨a, b⟩
 - apps ($a, b)
+
 -/
 
 inductive Expr where
@@ -114,19 +115,77 @@ inductive DefEq : Expr → Expr → Prop
   | right   : DefEq x x'  → DefEq ($ f, x) ($ f, x')
   | lleft   : DefEq a a'  → DefEq ⟪ a, b ⟫ ⟪ a', b ⟫
   | lright  : DefEq b b'  → DefEq ⟪ a, b ⟫ ⟪ a, b' ⟫
+  | nil_ctx : DefEq ⟪ ⟪ α, nil ⟫, Γ ⟫ ($ α, Γ)
 
 def id.type : Expr :=
-  ⟪ ⟪ ::[fst, fst], ::[fst, fst], ::[snd, fst] ⟫, ⟪ Ty, Ty ⟫ ⟫
+  ⟪ ⟪ fst, ::[fst, fst], ::[snd, fst], nil ⟫, ⟪ Ty, Ty ⟫ ⟫
 
-/-
-nil : ∀ (α : Type), α → Ty
--/
-def nil.type : Expr :=
-  ⟪ ⟪ ::[fst, fst], ::[fst, fst], ::[snd, snd, snd] ⟫, ⟪ Ty, Ty ⟫ ⟫
+def nil.type : Expr := Ty
 
 inductive ValidJudgment : Expr → Expr → Prop
-  | ty  : ValidJudgment Ty Ty
-  | app : ValidJudgment f ⟪ ⟪ α, β ⟫, Γ ⟫
+  | ty    : ValidJudgment Ty Ty
+  /-| comp : ValidJudgment g ⟪ ⟪ ($ α, Γ), ($ β, Γ), nil ⟫, Γ ⟫
+    → ValidJudgment f ⟪ ⟪ ($ β, Γ), Δ ⟫, Γ' ⟫
+    → ValidJudgment ::[f, g] ⟪ ⟪ α, ($ β, Γ), nil ⟫, Γ ⟫-/
+  | nil   : ValidJudgment nil nil.type
+  | app   : ValidJudgment f ⟪ ⟪ α, β ⟫, Γ ⟫
     → ValidJudgment x ($ α, Γ)
     → ValidJudgment ($ f, x) ⟪ β, ⟪ ⟪ x, ($ α, Γ) ⟫, Γ ⟫ ⟫
-  
+  | id    : ValidJudgment id id.type
+  | defeq : ValidJudgment x t₁
+    → DefEq t₁ t₂
+    → ValidJudgment x t₂
+
+syntax "defeq" ident,*        : tactic
+syntax "step" ident,*         : tactic
+syntax "judge" ident,*         : tactic
+
+macro_rules
+  | `(tactic| defeq $fn:ident,*) => do
+    let nms : Array (Lean.TSyntax `tactic) ← (Array.mk <$> (fn.getElems.toList.mapM (fun name =>
+      let nm := Lean.mkIdent (Lean.Name.mkStr `DefEq name.getId.toString)
+      `(tactic| apply $nm))))
+
+    `(tactic| $[$nms];*)
+  | `(tactic| step $fn:ident,*) => do
+    let nms : Array (Lean.TSyntax `tactic) ← (Array.mk <$> (fn.getElems.toList.mapM (fun name =>
+      let nm := Lean.mkIdent (Lean.Name.mkStr `IsStep name.getId.toString)
+      `(tactic| apply $nm))))
+
+    `(tactic| $[$nms];*)
+  | `(tactic| judge $fn:ident,*) => do
+    let nms : Array (Lean.TSyntax `tactic) ← (Array.mk <$> (fn.getElems.toList.mapM (fun name =>
+      let nm := Lean.mkIdent (Lean.Name.mkStr `ValidJudgment name.getId.toString)
+      `(tactic| apply $nm))))
+
+    `(tactic| $[$nms];*)
+
+theorem id_well_typed : ValidJudgment α Ty → ValidJudgment x α → ValidJudgment ($ id, α, x) α := by
+  intro h_t_α h_t_x
+  judge defeq, app, defeq, app, id, defeq
+  assumption
+  defeq symm, trans, step
+  step fst
+  defeq refl
+  defeq refl
+  judge defeq
+  assumption
+  defeq symm, trans, step
+  step comp
+  defeq trans, right, step
+  step fst
+  defeq step
+  step fst
+  defeq trans, nil_ctx, trans, step
+  step comp
+  defeq trans, right, step
+  step fst
+  defeq trans, step
+  step snd
+  defeq trans, step
+  step comp
+  defeq trans, right, step
+  step fst
+  defeq step
+  step fst
+
